extract tactics from tacSeq, setup initial tacs match

Struct/DevTest.lean
@@ -1,4 +1,5 @@
 import Struct.Struct
+import Struct.CustomTactics
 
 set_option pp.rawOnError true
 set_option trace.debug true
@@ -8,3 +9,43 @@ set_option trace.debug true
 --   structured simp
 --   structured cases n 
 --   case zero => sorry
+
+
+example (n : Nat) : true := by
+  cases n with
+  | zero => 
+    sorry
+  | succ n => 
+    sorry
+
+example (n : Nat) : true := by
+  induction n with
+  | zero => 
+    sorry
+  | succ n ih => 
+    sorry
+
+example : α → α := by
+  intro
+  -- fix (ha : α) ⊢ α
+  sorry
+example : α → α := by
+  intro ha
+  -- fix (ha : α) ⊢ α
+  sorry
+example : α → α := by
+  intros
+  -- fix (ha : α) ⊢ α
+  sorry
+example : α → β → α := by
+  intros ha hb
+  -- fix (ha : α) (hb : β) ⊢ α
+  sorry
+
+inductive Even : Nat → Prop
+| zero : Even Nat.zero
+| add_two : ∀ k : Nat, Even k → Even (k+2) 
+
+example : Even 0 := by
+  structured 
+    show Even 0 by apply Even.zero
