Struct/Struct.lean
@@ -12,112 +12,133 @@ open
   Lean.Parser 
   Lean.Parser.Tactic
 
-
 def structured (tacSeq : TSyntax ``tacticSeq) : TacticM Unit := do
-  -- TODO: Match on all our structures, ignore the rest
+  let tacs ← getTacs tacSeq
+
+  -- TODO : Match
+  match tacs with
+  | #[t] =>
+    addTrace `structured m!"This tactic is already structured"
+    evalTactic tacSeq
+
+  | _ =>
+
   -- match tacSeq with
   -- | `(tacticSeq|suffices $_ by $_) 
   -- | `(tacticSeq|show $_ by $_) 
   -- | `(tacticSeq|have $_ : $_ := by $_) 
+  -- | `(tacticSeq|clear $_)
   --   => 
   --   addTrace `structured m!"This tactic is already structured"
   --   evalTactic tacSeq
+  -- | `(tacticSeq|intro)
+  -- | `(tacticSeq|intro $id)
+  -- | `(tacticSeq|intros)
+  -- | `(tacticSeq|intros $ids*)
+  --   =>
+  --   addTrace `structured m!"Matched with intro, currently unimplemented"
+  --   evalTactic tacSeq
+  -- | `(tacticSeq|cases $_)
+  -- | `(tacticSeq|induction $_)
+  --   => 
+  --   addTrace `structured m!"Matched with cases or induction, currently unimplemented"
+  --   evalTactic tacSeq
   -- | _ => 
-  match (← getUnsolvedGoals) with
-  | [] => 
-    logWarning m!"No goals to solve, kind of shouldn't reach this, since we can't execute your tactic anyways"
-  | [goal] => 
-    let goalType ← instantiateMVars (← goal.getDecl).type
-    evalTactic tacSeq
     match (← getUnsolvedGoals) with
     | [] => 
-      let goalStx ← delab goalType
-      let stx ← mkShow goalStx tacSeq
-      addTrace `structured m!"Try this: {stx}"
-    | [newGoal] => 
-      let newGoalType ← instantiateMVars (← newGoal.getDecl).type
-      let isSameGoal := goalType.consumeMData == newGoalType.consumeMData
-
-      let lCtx := (← goal.getDecl).lctx
-      let lCtxNew := (← newGoal.getDecl).lctx
-
-      let declsNotInNew := diffLCtx lCtx lCtxNew
-      let declsNotInOld := diffLCtx lCtxNew lCtx
-
-      if !isSameGoal && declsNotInNew.size = 0 && declsNotInOld.size = 0 then
-        let newGoalStx ← delab (← instantiateMVars newGoalType)
-        let stx ← mkSuffices newGoalStx tacSeq
+      logWarning m!"No goals to solve, kind of shouldn't reach this, since we can't execute your tactic anyways"
+    | [goal] => 
+      let goalType ← instantiateMVars (← goal.getDecl).type
+      evalTactic tacSeq
+      match (← getUnsolvedGoals) with
+      | [] => 
+        let goalStx ← delab goalType
+        let stx ← mkShow goalStx tacSeq
         addTrace `structured m!"Try this: {stx}"
-      else if h : isSameGoal ∧ declsNotInNew.size = 0 ∧ declsNotInOld.size = 1 then
-        -- Prove that we know we can use the first index
-        have : 0 < declsNotInOld.size := by simp_all
-        let decl := declsNotInOld[0]
-        let declStx ← delab decl.type
-        -- NOTE: this stx does not really make sense, because from what I understand it can only happen if there is already a have clause
-        let newStx ← mkHave declStx tacSeq
-        addTrace `structured m!"Try this: {newStx}"
-      else
-        -- temp investigating types
-        -- let lCtx : LocalContext := (← goal.getDecl).lctx
-        -- for (decl : LocalDecl) in lCtx do
-        --   addTrace `structured m!"Decl Type : {decl.type}"
+      | [newGoal] => 
+        let newGoalType ← instantiateMVars (← newGoal.getDecl).type
+        let isSameGoal := goalType.consumeMData == newGoalType.consumeMData
 
-        --   -- Something with ConstantInfo, inductInfo
+        let lCtx := (← goal.getDecl).lctx
+        let lCtxNew := (← newGoal.getDecl).lctx
 
-        --   -- REALLY hacky way of ensuring we have the right decl we want to find constructors of
-        --   if toString decl.type == "Nat" then
-        --     let t : Expr := decl.type
-        --     addTrace `structured m!"Type Expression : {t}"
-        --     addTrace `structured m!"Expression Constructor : {Lean.Expr.ctorName t}"
-        --     match t with
-        --     | .const n us =>
-        --       addTrace `structured m!"Expression construcion with name : {n} and us {us}"
-        --       let x := (← getEnv).find? n
-        --       match x with 
-        --       | some (.inductInfo ival) => 
-        --         let ctors := ival.ctors
-        --       | _ => return
+        let declsNotInNew := diffLCtx lCtx lCtxNew
+        let declsNotInOld := diffLCtx lCtxNew lCtx
 
-        --     | _ =>
-        --       addTrace `structured m!"other"
+        if !isSameGoal && declsNotInNew.size = 0 && declsNotInOld.size = 0 then
+          let newGoalStx ← delab (← instantiateMVars newGoalType)
+          let stx ← mkSuffices newGoalStx tacSeq
+          addTrace `structured m!"Try this: {stx}"
+        else if h : isSameGoal ∧ declsNotInNew.size = 0 ∧ declsNotInOld.size = 1 then
+          -- Prove that we know we can use the first index
+          have : 0 < declsNotInOld.size := by simp_all
+          let decl := declsNotInOld[0]
+          let declStx ← delab decl.type
+          -- NOTE: this stx does not really make sense, because from what I understand it can only happen if there is already a have clause
+          let newStx ← mkHave declStx tacSeq
+          addTrace `structured m!"Try this: {newStx}"
+        else
+          -- temp investigating types
+          -- let lCtx : LocalContext := (← goal.getDecl).lctx
+          -- for (decl : LocalDecl) in lCtx do
+          --   addTrace `structured m!"Decl Type : {decl.type}"
 
-            -- TODO: how to get the existing known constructors of the const Nat
-            
-            -- Borrowed from Ed Ayers, but is not a match statement, doesnt use info on the type
-            -- let stx ← `(tactic| cases $(TSyntax.mk <| mkIdent localDecl.userName))
+          --   -- Something with ConstantInfo, inductInfo
 
-        -- end
-        logWarning m!"That combination of changes in goals and local declarations is currently unsupported 
-                      isSameGoal: {isSameGoal} {goalType} {newGoalType}
-                      NotInNew: {declsNotInNew.size} {declsNotInNew.map (fun x => x.type)} 
-                      NotInOld: {declsNotInOld.size} {declsNotInOld.map (fun x => x.type)}"
+          --   -- REALLY hacky way of ensuring we have the right decl we want to find constructors of
+          --   if toString decl.type == "Nat" then
+          --     let t : Expr := decl.type
+          --     addTrace `structured m!"Type Expression : {t}"
+          --     addTrace `structured m!"Expression Constructor : {Lean.Expr.ctorName t}"
+          --     match t with
+          --     | .const n us =>
+          --       addTrace `structured m!"Expression construcion with name : {n} and us {us}"
+          --       let x := (← getEnv).find? n
+          --       match x with 
+          --       | some (.inductInfo ival) => 
+          --         let ctors := ival.ctors
+          --       | _ => return
 
-    | newGoals => 
-      logWarning m!"Multiple goals after tactic execution, TODO to implement a case distinction suggestion"
-      -- temp for investigating case autocomplete
-      -- let mut cases := #[]
+          --     | _ =>
+          --       addTrace `structured m!"other"
 
-      -- for newGoal in newGoals do
-      --   let tag ← newGoal.getTag
-      --   let tseq ← `(tacticSeq|sorry)
-      --   let caseStx ← `(tactic|
-      --     case $(TSyntax.mk <| mkIdent tag):ident =>
-      --       $tseq:tacticSeq)
-      --   cases := cases.push caseStx
-      
-      -- -- TODO: Find neat way of unpacking cases
-      -- -- let firstCase := $cases[0]!
-      -- -- let allStx ← `(tacticSeq|
-      -- --   $tacSeq;
-      -- --   $firstCase)
+              -- TODO: how to get the existing known constructors of the const Nat
+              
+              -- Borrowed from Ed Ayers, but is not a match statement, doesnt use info on the type
+              -- let stx ← `(tactic| cases $(TSyntax.mk <| mkIdent localDecl.userName))
 
-      -- addTrace `structured m!"All Case Syntax combined : TODO"
-      -- -- end temp
+          -- end
+          logWarning m!"That combination of changes in goals and local declarations is currently unsupported 
+                        isSameGoal: {isSameGoal} {goalType} {newGoalType}
+                        NotInNew: {declsNotInNew.size} {declsNotInNew.map (fun x => x.type)} 
+                        NotInOld: {declsNotInOld.size} {declsNotInOld.map (fun x => x.type)}"
 
-  | goal::moreGoals =>
-    let goalDecl ← goal.getDecl
-    logWarning m!"Multiple goals pre-execution. This tactic may not work as expected if multiple goals change. Currently unimplemented"
-    evalTactic tacSeq
+      | newGoals => 
+        logWarning m!"Multiple goals after tactic execution, TODO to implement a case distinction suggestion"
+        -- temp for investigating case autocomplete
+        -- let mut cases := #[]
+
+        -- for newGoal in newGoals do
+        --   let tag ← newGoal.getTag
+        --   let tseq ← `(tacticSeq|sorry)
+        --   let caseStx ← `(tactic|
+        --     case $(TSyntax.mk <| mkIdent tag):ident =>
+        --       $tseq:tacticSeq)
+        --   cases := cases.push caseStx
+        
+        -- -- TODO: Find neat way of unpacking cases
+        -- -- let firstCase := $cases[0]!
+        -- -- let allStx ← `(tacticSeq|
+        -- --   $tacSeq;
+        -- --   $firstCase)
+
+        -- addTrace `structured m!"All Case Syntax combined : TODO"
+        -- -- end temp
+
+    | goal::moreGoals =>
+      let goalDecl ← goal.getDecl
+      logWarning m!"Multiple goals pre-execution. This tactic may not work as expected if multiple goals change. Currently unimplemented"
+      evalTactic tacSeq
 
 -- Elaborate tactic
 elab &"structured " t:tacticSeq : tactic =>
