Struct/Helpers.lean
@@ -7,6 +7,18 @@ open
   Lean.Parser.Tactic 
   Lean.Elab
 
+-- TODO: Create structure that completely determines changes before and after tacticSeq
+-- hasGoalChanged : Bool
+-- declsAdded : Array LocalDecl
+-- declsChanged : Array LocalDecl (or LocalDecl × LocalDecl if we need old one as well)
+-- .. TODO
+
+-- TODO: Create function that takes 2 `MVarId`s and constructs the change structure object
+
+-- TODO: Make Syntax object based on change structure object
+
+
+-- TODO: Refactor to `compareLCtx`, returning list of lostDecls, addedDecls, changedDecls
 -- TODO: Also check with usernames
 def diffLCtx (ctx₁ : LocalContext) (ctx₂: LocalContext) : Array LocalDecl := Id.run do
   let mut x := #[]
@@ -21,6 +33,11 @@ def diffLCtx (ctx₁ : LocalContext) (ctx₂: LocalContext) : Array LocalDecl :=
       x := x.push ldecl₁
   return x
 
+def getTacs (ts : TSyntax ``tacticSeq) : TermElabM (Array (TSyntax `tactic)) :=
+  match ts with
+  | `(tacticSeq| { $[$tacs:tactic $[;]?]* }) => return tacs
+  | `(tacticSeq| $[$tacs:tactic $[;]?]*) => return tacs
+  | _ => throwError "unknown syntax"
 
 -- Matches existing tacticSeq `ts` and appends tactic `t` at the end
 def mkTacticSeqAppend (ts : TSyntax ``tacticSeq) (t : TSyntax `tactic) : TermElabM (TSyntax ``tacticSeq) :=
@@ -45,7 +62,7 @@ def mkSuffices (t : Term) (tacSeq : TSyntax ``tacticSeq) : TermElabM (TSyntax ``
         $newTacSeq)
 
 -- def mkHave
-def mkHave (t : Term) (tacSeq : TSyntax ``tacticSeq) (n : Option Ident := none) : TermElabM (TSyntax ``tacticSeq) := do
+def mkHave (t : Term) (tacSeq : TSyntax ``tacticSeq) (n : Option Ident := none) : TermElabM (TSyntax ``tacticSeq) :=
   match n with
   | some name => 
     `(tacticSeq|
@@ -56,10 +73,19 @@ def mkHave (t : Term) (tacSeq : TSyntax ``tacticSeq) (n : Option Ident := none) 
       have : $t := by
         $tacSeq)
 
--- def mkChange
+-- def mkFix ... TODO from intro/intros
+
+-- def mkStrucNote ... TODO
 
 -- def mkCases
+-- def mkCases (target : TSyntax ``casesTarget) (cases : Array Term) : TermElabM (TSyntax ``tacticSeq) := do
+  -- match tacSeq with
+  -- | `(tactic|rfl) => sorry
+  -- | _ => sorry
+  -- let n : Term := _
+  -- let a ← `(tactic|
+  --   cases $target with
+  --   | $n => sorry)
+  -- sorry
 
 -- def mkInduction
-
--- #eval `(TSyntax.mk <| show 0 = 0 by rfl)
